handling ashr

coq/examples/test_16.c
@@ -5,14 +5,14 @@
 
 #include <klee/klee.h>
 
-//void test_ashr_1(int x) {
-//    int y = x >> 2;
-//}
-//
-//void test_ashr_2() {
-//    int x = klee_make_symbolic_int32();
-//    int y = x >> 7;
-//}
+void test_ashr_1(int x) {
+    int y = x >> 2;
+}
+
+void test_ashr_2() {
+    int x = klee_make_symbolic_int32();
+    int y = x >> 7;
+}
 
 void test_lshr_1(unsigned x) {
     unsigned y = x >> 2;
@@ -24,6 +24,8 @@ void test_lshr_2() {
 }
 
 int main() {
+    test_ashr_1(100);
+    test_ashr_2();
     test_lshr_1(100);
     test_lshr_2();
     return 0;
